RelationalAlgebra.lean
@@ -1,5 +1,5 @@
 -- This module serves as the root of the `RelationalAlgebra` library.
 -- Import modules here that should be built as part of the library.
 import RelationalAlgebra.RelationalModel
--- import RelationalAlgebra.RA.EquivRules
+import RelationalAlgebra.RA.EquivRules
 import RelationalAlgebra.FOL.ModelTheoryFOL
